CurryHowardCorrespondence/TypedLambda.lean
@@ -72,9 +72,17 @@ inductive Context : Type
 | Cons : VarName -> Types -> Context -> Context
 
 
-def Context.getType : Context → VarName → Types
-| Empty ,_ => Types.Empty
+def Context.getType : Context → VarName → Option Types
+| Empty ,_ => none
 | Cons x t Γ , y => if x == y then t else getType Γ y
+
+def eq_some_type : Option Types → Option Types → Bool
+| none , none => true
+| some _, none => false
+| none , some _ => false
+| some p, some q => p == q
+
+instance tseq: BEq (Option Types) := ⟨eq_some_type⟩
 
 def Context.IsSub: Context → Context → Bool
 | Empty, _ => true
@@ -90,7 +98,7 @@ instance : BEq Context := ⟨Context.BEq⟩
 
 
 inductive Inhabitable : Context → Types → Term → Prop
-| Var {Γ x A} (h : Γ.getType x == A) : Inhabitable Γ A (Term.Var x)
+| Var {Γ x A} (h : Γ.getType x == some A) : Inhabitable Γ A (Term.Var x)
 | Abs {Γ x A B t} (h : Inhabitable (Context.Cons x A Γ) B t) : Inhabitable Γ (Types.Arrow A B) (Term.Abs x A t)
 | App {Γ A B t1 t2} (h1 : Inhabitable Γ (Types.Arrow A B) t1) (h2 : Inhabitable Γ A t2) : Inhabitable Γ B (Term.App t1 t2)
 | Pair {Γ A B t1 t2} (h1 : Inhabitable Γ A t1) (h2 : Inhabitable Γ B t2) : Inhabitable Γ (Types.Touples A B) (Term.Pair t1 t2)
